WIP

secure_api/hkdf/Crypto.HMAC.fst
@@ -12,19 +12,28 @@ let wrap (a:alg) (key: bseq{Seq.length key <= maxLength a}):
   Tot (lbseq (blockLength a))
 = 
   let key0 = if length key <= blockLength a then key else hash a key in 
-  let padding = blockLength a - length key0 in 
-  key0 @| Seq.create padding 0uy
+  let paddingLength = blockLength a - length key0 in 
+  key0 @| Seq.create paddingLength 0uy
 
-noextract 
-let xor k v = Spec.Loops.seq_map (fun x -> FStar.UInt8.logxor x v) k
+private let wrap_lemma (a: alg) (key: bseq{Seq.length key <= maxLength a}): Lemma
+  (requires length key > blockLength a)
+  (ensures wrap a key == (
+    let key0 = hash a key in
+    let paddingLength = blockLength a - length key0 in 
+    key0 @| Seq.create paddingLength 0uy)) = ()
+
+noextract let rec xor (v: bseq) (x: UInt8.t): lbseq (length v) = 
+  init (length v) (fun i -> FStar.UInt8.logxor (index v i) x) 
+//  Spec.Loops.seq_map (fun y -> FStar.UInt8.logxor x y) v
+//18-04-08 not sure why the latter fails.
+
 
 // [noextract] incompatible with interfaces?!
 let hmac a key data =
   let k = wrap a key in 
-  let h1 = hash a (xor k 0x36uy @| data) in 
-  let h2 = hash a (xor k 0x5cuy @| h1) in 
+  let h1 = spec a (xor k 0x36uy @| data) in 
+  let h2 = spec a (xor k 0x5cuy @| h1) in 
   h2
-
 
 /// Agile implementation, relying on using 3 variants of SHA2
 /// supported by HACL*.
@@ -35,10 +44,7 @@ open FStar.UInt32
 
 module ST = FStar.HyperStack.ST
 
-// ADL lax prototype for QUIC deadline
-// 18-03-04 restructured
-
-(* we rely on the output being zero-initialized in case the key is less than a block *)
+(* we rely on the output being zero-initialized for the correctness of padding *)
 [@"substitute"]
 val wrap_key:
   a: alg ->
@@ -55,237 +61,133 @@ val wrap_key:
       modifies_1 output h0 h1 /\
       as_seq h1 output = wrap a (as_seq h0 key) ))
 
-// replaced by [H.compute]; not sure why it required pre-zeroing-out the result.
-// let agile_hash (a:alg) (output:uint8_p{length output = tagLength a})
-//   (input:uint8_p{length input < maxLength a /\ disjoint output input})
-//   (len:uint32_t{v len = length output})
-//   : Stack unit
-//   (requires fun h -> live h input /\ live h output
-//     /\ (as_seq h output) == Seq.create (tagLength a) 0uy)
-//   (ensures fun h0 () h1 -> live h1 output /\ live h1 input
-//     /\ modifies_1 output h0 h1
-//     /\ as_seq h1 input == as_seq h0 input
-//     /\ correct_agile_hash a (as_seq h1 input) (as_seq h1 output))
-//   =
-//   match a with
-//   | SHA256 -> Hacl.Hash.SHA2_256.hash output input len
-//   | SHA384 -> Hacl.Hash.SHA2_384.hash output input len
-//   | SHA512 -> Hacl.Hash.SHA2_512..hash output input len
-
-//#reset-options "--max_fuel 0  --z3rlimit 250"
 [@"substitute"]
 let wrap_key a output key len =
- (**) let h0 = ST.get () in
-  if len <=^ blockLen a then
-   begin
-    (**) assert(v (blockLen a) - v len >= 0);
-    (**) assert(as_seq h0 output == Seq.create (v (blockLen a)) 0uy);
-    Buffer.blit key 0ul output 0ul len;
-    (**) let h1 = ST.get () in
-    (**) Seq.lemma_eq_intro (Seq.slice (as_seq h1 output) 0 (v len)) (as_seq h0 key);
-    (**) assert(Seq.slice (as_seq h1 output) 0 (v len) == as_seq h0 key);
-    (**) Seq.lemma_eq_intro (Seq.slice (as_seq h1 output) (v len) (v (blockLen a))) (Seq.create (v (blockLen a) - v len) 0uy);
-    (**) assert(Seq.slice (as_seq h1 output) (v len) (v (blockLen a)) == Seq.create (v (blockLen a) - v len) 0uy);
-    (**) Seq.lemma_eq_intro (as_seq h1 output) (Seq.append (as_seq h0 key) (Seq.create (v (blockLen a) - v len) 0uy));
-    (**) assert(as_seq h1 output == Seq.append (as_seq h0 key) (Seq.create (v (blockLen a) - v len) 0uy))
-   end
-  else
-   begin
-    (**) assert(v (blockLen a) - tagLength a >= 0);
-    (**) assert(as_seq h0 output == Seq.create (v (blockLen a)) 0uy);
-    (**) Seq.lemma_eq_intro (Seq.slice (as_seq h0 output) 0 (tagLength a)) (Seq.create (tagLength a) 0uy);
-    (**) assert(Seq.slice (as_seq h0 output) 0 (tagLength a) == Seq.create (tagLength a) 0uy);
-    (**) Seq.lemma_eq_intro (Seq.slice (as_seq h0 output) (tagLength a) (v (blockLen a))) (Seq.create (v (blockLen a) - tagLength a) 0uy);
-    (**) assert(Seq.slice (as_seq h0 output) (tagLength a) (v (blockLen a)) == Seq.create (v (blockLen a) - tagLength a) 0uy);
-    let nkey = Buffer.sub output 0ul (tagLen a) in
-    Hash.compute a len key nkey
-    (**) //let h1' = ST.get () in
-    (**) //assert(as_seq h1' nkey == );
-    (**) //assert(Seq.slice (as_seq h1' output) 0 (tagLength a) == Spec_Hash.hash (as_seq h0 key));
-    (**) //no_upd_lemma_1 h0 h1' (Buffer.sub output 0ul (tagLen a)) (Buffer.sub output (tagLen a) blockLen a) -^ (tagLen a)));
-    (**) //Seq.lemma_eq_intro (Seq.slice (reveal_sbytes (as_seq h1' output)) (tagLength a) (v (blockLen )) (Seq.create (v (blockLen a) - tagLength a) 0uy);
-    (**) //assert(Seq.slice (reveal_sbytes (as_seq h1' output)) (tagLength a) (v (blockLen a)) == Seq.create (v (blockLen a) - tagLength a) 0uy);
-    (**) //Seq.lemma_eq_intro (reveal_sbytes (as_seq h1' output)) (Seq.append (reveal_sbytes (as_seq h1' nkey)) (Seq.create (v (blockLen a) - tagLength a) 0uy));
-    (**) //assert(reveal_sbytes (as_seq h1' output) == Seq.append (reveal_sbytes (as_seq h1' nkey)) (Seq.create (v (blockLen a) - tagLength a) 0uy))
-   end
+  let i = if len <=^ blockLen a then len else tagLen a in 
+  let nkey = Buffer.sub output 0ul i in 
+  let pad = Buffer.sub output i (blockLen a -^ i) in
+  let h0 = ST.get () in
+  if len <=^ blockLen a then 
+    Buffer.blit key 0ul nkey 0ul len
+  else 
+    Hash.compute a len key nkey;
+  let h1 = ST.get () in
+  Seq.lemma_eq_intro (as_seq h0 pad) (Seq.create (blockLength a - v i) 0uy);
+  Seq.lemma_split (as_seq h1 output) (v i)
 
-(* should not be necessary 
-//#reset-options " --initial_fuel 1 --max_fuel 1 --initial_ifuel 1 --max_ifuel 1 --z3rlimit 10"
-let counter_pos: alg -> Tot uint32_t = function
-  | SHA256 -> Hacl.Hash.SHA2_256.pos_count_w
-  | SHA384 -> Hacl.Hash.SHA2_384.pos_count_w
-  | SHA512 -> Hacl.Hash.SHA2_512.pos_count_w
-
-//#reset-options "--initial_fuel 1 --max_fuel 1 --initial_ifuel 1 --max_ifuel 1 --z3rlimit 10"
-let counter_size: alg -> Tot uint32_t = function
-  | SHA256 -> Hacl.Hash.SHA2_256.size_count_w
-  | SHA384 -> Hacl.Hash.SHA2_384.size_count_w
-  | SHA512 -> Hacl.Hash.SHA2_512..size_count_w
-*)
-
-(* usage? 
-//#reset-options "--max_fuel 0  --z3rlimit 50"
-val lemma_alloc:
-  a: alg ->
-  s: state a ->
-  Lemma
-    (requires (s == Seq.create (v (state_size a)) 0ul))
-    (ensures (
-      let seq_counter = Seq.slice s (U32.v (counter_pos a)) (U32.(v (counter_pos a) + v (counter_size a))) in
-      let counter = Seq.index seq_counter 0 in
-      U32.v counter = 0))
-let lemma_alloc a s = ()
-*)
-
-//#reset-options "--max_fuel 0  --z3rlimit 20"
 [@"substitute"]
-val hmac_part1:
+val part1:
   a: alg ->
   s2: lbptr (blockLength a) ->
-  data: bptr {length data + blockLength a  < pow2 32 /\ disjoint data s2} ->
+  data: bptr {
+    length data + blockLength a  < pow2 32 /\ 
+    length data + blockLength a  <= maxLength a /\ 
+    disjoint data s2} ->
   len: UInt32.t {length data = v len} ->
   Stack unit
-        (requires (fun h0 ->  live h0 s2 /\ live h0 data))
-        (ensures  (fun h0 _ h1 -> live h1 s2 /\ live h0 s2
-                             /\ live h1 data /\ live h0 data /\ modifies_1 s2 h0 h1
-                             /\ (let hash0 = Seq.slice (as_seq h1 s2) 0 (tagLength a) in
-                             hash0 = hash a (Seq.append (as_seq h0 s2) (as_seq h0 data)))))
+    (requires (fun h0 ->  live h0 s2 /\ live h0 data))
+    (ensures  (fun h0 _ h1 -> 
+      live h1 s2 /\ live h0 s2 /\ live h1 data /\ live h0 data /\ modifies_1 s2 h0 h1 /\ (
+      let hash0 = Seq.slice (as_seq h1 s2) 0 (tagLength a) in
+      hash0 == spec a (Seq.append (as_seq h0 s2) (as_seq h0 data)))))
 
-(*
-let agile_alloc (a:alg) : Stack (st:state a)
-  (requires fun h -> True)
-  (ensures fun h0 () h1 -> True)
-  =
-  match a with
-  | SHA256 -> Buffer.create 0ul (state_size a)
-  | SHA384 -> Buffer.create 0uL (state_size a)
-  | SHA512 -> Buffer.create 0uL (state_size a)
-*)
-
-//18-03-04 the condition on len was probably false; not also the
-//calling convention has changed.
-// let Hash.update_last (a:alg) (st:state a)
-//   (input:uint8_p {length input = v (blockLen a)})
-//   (len:uint32_t {v len = length input})
-//   : Stack unit (requires fun h -> True)
-//   (ensures fun h0 () h1 -> True)
-//    //live h1 st /\ modifies_1 st h0 h1)
-//   =
-//   match a with
-//   | SHA256 -> Hacl.Hash.SHA2_256.update_last st input len
-//   | SHA384 -> Hacl.Hash.SHA2_384.update_last st input (Int.Cast.uint32_to_uint64 len)
-//   | SHA512 -> Hacl.Hash.SHA2_512..update_last st input (Int.Cast.uint32_to_uint64 len)
-
-
-//#reset-options "--max_fuel 0  --z3rlimit 200"
+#reset-options "--max_fuel 0 --z3rlimit 200"
 [@"substitute"]
-let hmac_part1 a s2 data len =
-
-  (* Push a new memory frame *)
-  (**) push_frame ();
-  (**) let h0 = ST.get () in
-
-  (* Allocate memory for the Hash function state *)
-  // let state0 = Hash.alloc () in
-  let state0 = Buffer.create 0ul (state_size a) in
-  (**) let h = ST.get() in
-  (**) //lemma_alloc (reveal_h32s (as_seq h state0));
-  (**) no_upd_lemma_0 h0 h s2;
-  (**) no_upd_lemma_0 h0 h data;
-
-  (* Step 3: append data to "result of step 2" *)
-  (* Step 4: apply Hash to "result of step 3" *)
-  (**) assert((blockLen a) <> 0ul);
-  (**) Math.Lemmas.lemma_div_mod (v len) (v (blockLen a));
+let part1 a keyblock data len =
+  push_frame ();
+  // 18-04-09 monomorphic; otherwise verification dies
+  if a = SHA256 then (
+  // 18-04-09 Kremlin complains about variable-size allocation, 
+  // why? can we force normalization? [normalize_term] does not help.
+  let acc = Buffer.create 0ul (state_size a) in
+  Math.Lemmas.lemma_div_mod (v len) (blockLength a);
   let n0 = len /^ blockLen a in
   let r0 = len %^ blockLen a in
-  let blocks0 = Buffer.sub data 0ul (n0 *^ (blockLen a)) in
-  let last0 = Buffer.offset data (n0 *^ (blockLen a)) in
-  (**) Seq.lemma_eq_intro (Seq.slice (as_seq h data) 0 (UInt32.v (n0 *^ (blockLen a)))) (as_seq h blocks0);
-  (**) Seq.lemma_eq_intro (Seq.slice (as_seq h data) (UInt32.v (n0 *^ (blockLen a))) (length data)) (as_seq h last0);
-  Hash.init a state0;  
-  (**) //let h' = ST.get() in
-  (**) //no_upd_lemma_1 h h' state0 s2;
-  (**) //no_upd_lemma_1 h h' state0 data;
-  (**) //no_upd_lemma_1 h h' state0 blocks0;
-  (**) //no_upd_lemma_1 h h' state0 last0;
-  Hash.update a state0 s2;
-  (**) //let h'' = ST.get() in
-  (**) //no_upd_lemma_1 h' h'' state0 blocks0;
-  (**) //no_upd_lemma_1 h' h'' state0 last0;
-  Hash.update_multi a state0 blocks0 n0;
-  (**) //let h''' = ST.get() in
-  (**) //no_upd_lemma_1 h'' h''' state0 last0;
-  Hash.update_last a state0 last0 len;
-  (**) let h1 = ST.get () in
+  let data_blocks = Buffer.sub data 0ul (n0 *^ blockLen a) in
+  let data_last = Buffer.offset data (n0 *^ blockLen a) in
+  Hash.init a acc;  
+  Hash.update a acc keyblock;
+  let h1 = ST.get() in 
+  Hash.update_multi a acc data_blocks (n0 *^ blockLen a);
+  let h2 = ST.get() in
+  Hash.update_last a acc data_last (blockLen a +^ len);
+  let h3 = ST.get() in
+  let tag = Buffer.sub keyblock 0ul (tagLen a) in (* Salvage memory *)
+  Hash.extract a acc tag; 
+  (
+    let v1 = as_seq h1 keyblock in 
+    let vblocks = as_seq h1 data_blocks in 
+    let acc1 = as_acc h1 acc in 
+    lemma_compress (acc0 #a) v1;
+    assert(acc1 == hash0 #a v1);
+    let v2 = v1 @| vblocks in 
+    let acc2 = as_acc h2 acc in 
+    lemma_hash2 (acc0 #a) v1 vblocks;
+    assert(acc2 == hash0 #a v2);
+    let vdata = as_seq h1 data in  
+    let vlast = as_seq h1 data_last in 
+    let vsuffix = suffix a (blockLength a + v len) in 
+    Seq.lemma_eq_intro vdata (vblocks @| vlast);
+    let acc3 = as_acc h3 acc in 
+    lemma_hash2 (acc0 #a) v2 (vlast @| vsuffix); 
+    assert(acc3 == hash0 #a (v2 @| (vlast @| vsuffix)));
+    Seq.append_assoc v2 vlast vsuffix; 
+    Seq.append_assoc v1 vblocks vlast;
+    assert(acc3 == hash0 #a ((v1 @| vdata) @| vsuffix));
+    assert(finish acc3 == spec a (v1 @| vdata))
+  ))
+  else admit();
+  pop_frame()
 
-  let h'''' = ST.get() in
-  let hash0 = Buffer.sub s2 0ul (tagLen a) in (* Salvage memory *)
-  Hash.extract a state0 hash0; (* s4 = hash (s2 @| data) *)
-//  (**) Spec_Hash.lemma_hash_all_prepend_block (reveal_sbytes (as_seq h0 s2)) (reveal_sbytes (as_seq h0 data));
-
-  (* Pop the memory frame *)
-  (**) pop_frame ()
-
-
-//#reset-options "--max_fuel 0  --z3rlimit 20"
+// the two parts have the same stucture; let's keep their proofs in sync. 
+  
 [@"substitute"]
-val hmac_part2:
+val part2:
   a: alg ->
   mac: lbptr (tagLength a) ->
-  s5: lbptr (blockLength a) {disjoint s5 mac} ->
-  s4: lbptr (tagLength a) {disjoint s4 mac /\ disjoint s4 s5} ->
+  opad: lbptr (blockLength a) ->
+  tag: lbptr (tagLength a) {disjoint mac opad /\ disjoint mac tag} ->
   Stack unit
-        (requires (fun h -> True)) //live h mac /\ live h s5 /\ live h s4))
-        (ensures  (fun h0 _ h1 -> live h1 mac /\ live h0 mac))
+    (requires fun h -> live h mac /\ live h opad /\ live h tag)
+    (ensures fun h0 _ h1 -> 
+      live h1 mac /\ live h0 mac /\ modifies_1 mac h0 h1 /\
+      ( let payload = Seq.append (as_seq h0 opad) (as_seq h0 tag) in 
+        Seq.length payload <= maxLength a /\
+        as_seq h1 mac = spec a payload))
+
  //TODO spec
  ///\ live h1 s5 /\ live h0 s5
  ///\ live h1 s4 /\ live h0 s4 /\ modifies_1 mac h0 h1
  ///\ (reveal_sbytes (as_seq h1 mac) == Spec_Hash.hash (Seq.append (reveal_sbytes (as_seq h0 s5)) (reveal_sbytes (as_seq h0 s4))))))
 
-//#reset-options "--max_fuel 0  --z3rlimit 200"
 [@"substitute"]
-let hmac_part2 a mac s5 s4 =
-  (**) assert_norm(pow2 32 = 0x100000000);
-  (**) let hinit = ST.get() in
-  (**) push_frame ();
-  (**) let h0 = ST.get () in
-  (* Allocate memory for the Hash function state *)
-  (* let state1 = Hash.alloc () in *)
-  let state1 = Buffer.create 0ul (state_size a) in
-
-  (* Step 6: append "result of step 4" to "result of step 5" *)
-  (* Step 7: apply H to "result of step 6" *)
-  (**) let h = ST.get() in
-  (**) no_upd_lemma_0 h0 h s5;
-  (**) no_upd_lemma_0 h0 h s4;
-  (**) no_upd_lemma_0 h0 h mac;
-  (**) //lemma_alloc (reveal_h32s (as_seq h state1));
-  Hash.init a state1;
-  (**) let h' = ST.get() in
-  (**) //assert(let st_h0 = Seq.slice (as_seq h' state1) (U32.v Hash.pos_whash_w) (U32.(v Hash.pos_whash_w + v Hash.size_whash_w)) in
-  (**) //reveal_h32s st_h0 == Spec_Hash.h_0);
-  (**) no_upd_lemma_1 h h' state1 s5;
-  (**) no_upd_lemma_1 h h' state1 s4;
-  (**) no_upd_lemma_1 h h' state1 mac;
-  Hash.update a state1 s5; (* s5 = opad *)
-  (**) let h'' = ST.get() in
-  (**) //assert(let st_h0 = Seq.slice (as_seq h'' state1) (U32.v Hash.pos_whash_w) (U32.(v Hash.pos_whash_w + v Hash.size_whash_w)) in
-  (**) //       reveal_h32s st_h0 == Spec_Hash.(update h_0 (reveal_sbytes (as_seq h0 s5))));
-  (**) no_upd_lemma_1 h' h'' state1 s4;
-  (**) no_upd_lemma_1 h' h'' state1 mac;
-  (**) assert(as_seq h'' s4 == as_seq hinit s4);
-  Hash.update_last a state1 s4 (blockLen a +^ tagLen a);
-  (**) let h''' = ST.get() in
-  (**) no_upd_lemma_1 h' h'' state1 s4;
-  (**) no_upd_lemma_1 h' h'' state1 mac;
-  (**) assert(live h''' mac);
-  Hash.extract a state1 mac; //(* s7 = hash (s5 @| s4) *)
-  (**) //let h1 = ST.get() in
-  (**) //Spec_Hash.lemma_hash_single_prepend_block (reveal_sbytes (as_seq h0 s5)) (reveal_sbytes (as_seq h0 s4));
-  (**)  //Seq.lemma_eq_intro (reveal_sbytes (as_seq h1 mac)) (Spec_Hash.hash (Seq.append (reveal_sbytes (as_seq h0 s5)) (reveal_sbytes (as_seq h0 s4))));
-  (**) //assert(reveal_sbytes (as_seq h1 mac) == Spec_Hash.hash (Seq.append (reveal_sbytes (as_seq h0 s5)) (reveal_sbytes (as_seq h0 s4))));
-  (**) pop_frame ()
+let part2 a mac opad tag =
+  push_frame ();
+  if a = SHA256 then (
+  let totLen = blockLen a +^ tagLen a in 
+  assert_norm(v totLen <= maxLength a);
+  let acc = Buffer.create 0ul (state_size a) in
+  Hash.init a acc;
+  Hash.update a acc opad; 
+  let h1 = ST.get() in 
+  Hash.update_last a acc tag totLen;
+  let h2 = ST.get() in 
+  Hash.extract a acc mac;
+  (
+    let v1 = as_seq h1 opad in
+    let acc1 = as_acc h1 acc in 
+    lemma_compress (acc0 #a) v1;
+    assert(acc1 == hash0 #a v1);
+    let vtag = as_seq h1 tag in 
+    let vsuffix = suffix a (blockLength a + tagLength a) in
+    let acc2 = as_acc h2 acc in 
+    lemma_hash2 (acc0 #a) v1 (vtag @| vsuffix); 
+    Seq.append_assoc v1 vtag vsuffix;
+    assert(acc2 == hash0 #a ((v1 @| vtag) @| vsuffix));
+    assert(finish acc2 = spec a (v1 @| vtag))
+  )) 
+  else admit(); 
+  pop_frame ()
 
 (* same spec as hmac with keylen = blockLen a *)
 //#reset-options "--max_fuel 0  --z3rlimit 20"
@@ -293,64 +195,66 @@ val hmac_core:
   a: alg ->
   tag: lbptr (tagLength a) ->
   key: lbptr (blockLength a) {disjoint key tag} ->
-  data: bptr {length data + blockLength a < pow2 32 /\ disjoint data tag /\ disjoint data key} ->
+  data: bptr {
+    length data + blockLength a < pow2 32 /\ 
+    length data + blockLength a <= maxLength a /\
+    disjoint data tag /\ disjoint data key} ->
   datalen: UInt32.t {v datalen = length data} ->
   Stack unit
-  (requires (fun h0 -> live h0 tag /\ live h0 key /\ live h0 data))
-  (ensures  (fun h0 _ h1 -> 
+  (requires fun h0 -> live h0 tag /\ live h0 key /\ live h0 data)
+  (ensures fun h0 _ h1 -> 
     live h1 tag /\ live h0 tag /\
     live h1 key /\ live h0 key /\
-    live h1 data /\ live h0 data /\ modifies_1 tag h0 h1 /\
-    as_seq h1 tag = hmac a (as_seq h0 key) (as_seq h0 data)))
+    live h1 data /\ live h0 data /\ //18-04-08 TODO modifies_1 tag h0 h1 /\
+    ( let k = as_seq h0 key in  
+      let k1 = xor k 0x36uy in
+      let k2 = xor k 0x5cuy in
+      let v1 = spec a (k1 @| as_seq h0 data) in 
+      Seq.length (k2 @| v1) <= maxLength a /\
+      as_seq h1 tag = spec a (k2 @| v1)))
+      //harder: hmac a (as_seq h0 key) (as_seq h0 data)
 
 //#reset-options "--max_fuel 0 --z3rlimit 10"
 let xor_bytes_inplace a b len =
   C.Loops.in_place_map2 a b len (fun x y -> UInt8.logxor x y)
 // below, we only XOR with a constant bytemask.
 
-//#reset-options "--max_fuel 0  --z3rlimit 150"
 let hmac_core a mac key data len =
-  (**) let h00 = ST.get () in
-  (**) push_frame ();
-  (**) let h0 = ST.get () in
-/// 18-03-03 avoid those and do the xor on copying?
-  (* Initialize constants *)
+  push_frame ();
   let ipad = Buffer.create 0x36uy (blockLen a) in
   let opad = Buffer.create 0x5cuy (blockLen a) in
-  (**) let h1 = ST.get () in
-  (**) //assert(reveal_sbytes (as_seq h1 ipad) == Seq.create (v (blockLen a)) 0x36uy);
-  (**) //assert(reveal_sbytes (as_seq h1 opad) == Seq.create (v (blockLen a)) 0x5cuy);
-
-  (* Step 2: xor "result of step 1" with ipad *)
   xor_bytes_inplace ipad key (blockLen a);
-  (**) let h2 = ST.get () in
-  (**) //assert(reveal_sbytes (as_seq h2 ipad) == Spec.xor_bytes (reveal_sbytes (as_seq h1 ipad)) (reveal_sbytes (as_seq h0 key)));
-
-  (* Step 3: append data to "result of step 2" *)
-  (* Step 4: apply Hash to "result of step 3" *)
-  hmac_part1 a ipad data len; (* s2 = ipad *)
-  let s4 = Buffer.sub ipad 0ul (tagLen a) in (* Salvage memory *)
-  (**) let h3 = ST.get () in
-  (**) //Seq.lemma_eq_intro (as_seq h3 (Buffer.sub ipad 0ul (tagLen a))) (Seq.slice (as_seq h3 ipad) 0 (tagLength a));
-  (**) //assert(reveal_sbytes (as_seq h3 s4) == Spec_Hash.hash (Seq.append (reveal_sbytes (as_seq h2 ipad)) (reveal_sbytes (as_seq h0 data))));
-  (**) //assert(reveal_sbytes (as_seq h3 s4) == Spec_Hash.hash (Seq.append (Spec.xor_bytes (reveal_sbytes (as_seq h1 ipad)) (reveal_sbytes (as_seq h0 key))) (reveal_sbytes (as_seq h0 data))));
-
-  (* Step 5: xor "result of step 1" with opad *)
   xor_bytes_inplace opad key (blockLen a);
-  (**) let h4 = ST.get () in
-  (**) //assert(reveal_sbytes (as_seq h4 opad) == Spec.xor_bytes (reveal_sbytes (as_seq h1 opad)) (reveal_sbytes (as_seq h0 key)));
+  // in principle, we can re-use the same pad for both, xoring it with
+  // (0x36uy xor 0x5cuy) in-between.
+  let h0 = ST.get() in
+  part1 a ipad data len; 
+  let h1 = ST.get() in 
+  let inner = Buffer.sub ipad 0ul (tagLen a) in (* Salvage memory *)
+  part2 a mac opad inner;
+  let h2 = ST.get() in 
+  ( 
+    let k = as_seq h0 key in  
+    let k1: lbseq (blockLength a) = xor k 0x36uy in
+    let k2: lbseq (blockLength a) = xor k 0x5cuy in
+    let vdata = as_seq h0 data in 
+    let v1: lbseq (tagLength a) = as_seq h1 inner in 
+    assert_norm(blockLength a + tagLength a <= maxLength a);
+    assert(Seq.length (k2 @| v1) <= maxLength a);
+    let v2 = as_seq h2 mac in 
+    assume(as_seq h0 ipad = k1);
+    assume(as_seq h1 opad = k2);
+    assert(v1 == spec a (k1 @| vdata));
+    assert(v2 == spec a (k2 @| v1)));
+  pop_frame ()
 
-  (* Step 6: append "result of step 4" to "result of step 5" *)
-  (* Step 7: apply H to "result of step 6" *)
-  hmac_part2 a mac opad s4; (* s5 = opad *)
-  (**) let h5 = ST.get () in
-  (**) //assert(reveal_sbytes (as_seq h5 mac) == Spec.hmac_core (reveal_sbytes (as_seq h0 key)) (reveal_sbytes (as_seq h0 data)));
-  (**) pop_frame ()
+// not much point in separating hmac_core (verbose spec)
 
-//#reset-options "--max_fuel 0  --z3rlimit 25"
 let compute a mac key keylen data datalen =
   push_frame (); 
-  let wrapped_key = Buffer.create 0x00uy (blockLen a) in
-  wrap_key a wrapped_key key keylen;
-  hmac_core a mac wrapped_key data datalen;
+  let keyblock = Buffer.create 0x00uy (blockLen a) in
+  assert_norm(pow2 32 <= maxLength a);
+  wrap_key a keyblock key keylen;
+  hmac_core a mac keyblock data datalen;
   pop_frame ()
+
