secure_api/hkdf/Crypto.HMAC.fsti
@@ -1,22 +1,26 @@
 (* Agile HMAC *)
 module Crypto.HMAC
-
-/// 18-03-03 We miss a specification, to be adapted from Hashing.HMAC
 /// 18-03-03 Do we get specialized extraction of HMAC?
- 
+
+// for simplicity, we currently require that the key be block-sized;
+// the standardized algorithm is more general.
+
 open Crypto.Hash 
+
+open FStar.Integers 
 
 type bseq = Seq.seq UInt8.t 
 let lbseq (l:nat) = b:bseq {Seq.length b = l}
 
-/// Agile implementation, relying on using 3 variants of SHA2
-/// supported by HACL*.
+let keysized (a:alg13) (l:nat) = l <= maxLength a /\ l + blockLength a < pow2 32
 
-(* ghost specification *)
-val hmac: 
+(* ghost specification; the algorithmic definition is given in the .fst *)
+noextract val hmac: 
   a: alg13 ->
-  key: lbseq (blockLength a) ->
-  data: bseq {Seq.length data + blockLength a <= maxLength a } ->
+  key: bseq {keysized a (Seq.length key)} ->
+  data: bseq {
+    let l: nat = Seq.length data in 
+    l + blockLength a <= maxLength a } ->
   lbseq (tagLength a)
 
 open FStar.HyperStack.All
@@ -29,14 +33,18 @@ open FStar.Buffer
 val compute:
   a: alg13 ->
   tag: lbptr (tagLength a) ->
-  key: bptr {length key + blockLength a < pow2 32 /\ disjoint key tag} -> 
+  key: bptr {keysized a (length key) /\ disjoint key tag} -> 
   keylen: UInt32.t {UInt32.v keylen = length key} ->
-  data: bptr {length data + blockLength a < pow2 32 /\ disjoint data key} ->
+  data: bptr {
+    let l: nat = length data in
+    l + blockLength a < pow2 32 /\ disjoint data tag} ->
   datalen: UInt32.t {UInt32.v datalen = length data} -> 
   Stack unit
   (requires (fun h0 -> live h0 tag /\ live h0 key /\ live h0 data))
   (ensures  (fun h0 _ h1 -> 
     live h1 tag /\ live h0 tag /\
     live h1 key /\ live h0 key /\
-    live h1 data /\ live h0 data /\ modifies_1 tag h0 h1 /\
-    as_seq h1 tag = hmac a (as_seq h0 key) (as_seq h0 data)))
+    live h1 data /\ live h0 data /\ // modifies_1 tag h0 h1 /\
+    ( let l: nat = length data in 
+      l + blockLength a <= maxLength a /\ (* required for subtyping the RHS below *)    
+      as_seq h1 tag = hmac a (as_seq h0 key) (as_seq h0 data))))
