secure_api/hkdf/Crypto.Hash.fsti
@@ -13,9 +13,6 @@ open FStar.HyperStack.ST
 type bseq = Seq.seq UInt8.t 
 let lbseq (l:nat) = b:bseq {Seq.length b = l}
 
-// we also have FStar's bytes and lbytes 
-
-
 (* SUPPORTED ALGORITHMS; the first 3 are still required by TLS 1.2,
    included for legacy purpose only, and not provided by HACL*.  See
    e.g. https://en.wikipedia.org/wiki/SHA-1 for a global comparison
@@ -45,12 +42,6 @@ let blockLen = function
 noextract 
 let blockLength a = UInt32.v (blockLen a)
 
-let lemma_blockLengths = 
-  assert_norm(
-    blockLength SHA256 == Spec.SHA2_256.size_block /\
-    blockLength SHA384 == Spec.SHA2_384.size_block /\
-    blockLength SHA512 == Spec.SHA2_512.size_block)
-
 (* RESULT TAGS and their lengths, in bytes *)
 
 let maxTagLen = 64ul
@@ -70,21 +61,9 @@ let lbytes l = b:Bytes.bytes {Bytes.length b = l}
 type tag (a:alg) = b: lbytes (tagLength a)
 type anyTag = lbytes (v maxTagLen)
 
-noextract let lemma_tagLengths = 
-  assert_norm(
-    tagLength SHA256 == Spec.SHA2_256.size_hash /\
-    // truncated SHA512; note that `size_hash` is 64, not 48
-    tagLength SHA384 == Spec.SHA2_384.(size_word `op_Multiply` size_hash_final_w) /\
-    tagLength SHA512 == Spec.SHA2_512.size_hash)
+// to be imported from HACL* 
+noextract let maxLength: alg -> nat = fun a -> pow2 61 - 1 
 
-//#reset-options "--initial_ifuel 2 --initial_fuel 2 --z3rlimit 30"
-(* maximal input size, in bytes *)
-noextract let maxLength: alg -> nat = function
-  // 18-03-02 hacl-star uses a strict inequality; why?
-  | SHA256 -> Spec.SHA2_256.max_input_len_8 - 1 
-  | SHA384 -> Spec.SHA2_384.max_input_len_8 - 1 
-  | SHA512 -> Spec.SHA2_512.max_input_len_8 - 1
-  | _      -> pow2 61 (* conservative *)
 noextract let lemma_maxLength (a:alg13) = assert_norm (pow2 32 <= maxLength a) 
 noextract let hashable (a:alg) = b: bseq{ Seq.length b <= maxLength a }
 
@@ -92,17 +71,17 @@ noextract let hashable (a:alg) = b: bseq{ Seq.length b <= maxLength a }
    algorithms for all byte lengths; used for aligning specs and
    implementations but irrelevant for using hashes.  *)
 
-val acc (a:alg): Type0 (*noeq*)
+noextract val acc (a:alg): Type0 // noeq, but `noeq val` is not supported)
 
 (* sets the initial value of the accumulator *) 
-val acc0: #a:alg -> acc a 
+noextract val acc0: #a:alg -> acc a 
 
 (* hashes one block of data into the accumulator *)
-val compress: #a:alg -> acc a -> b: lbseq (blockLength a) -> acc a 
+noextract val compress: #a:alg -> acc a -> b: lbseq (blockLength a) -> acc a 
 
 (* extracts the tag from the (possibly larger) accumulator *)
-val finish: #a:alg -> acc a -> lbseq (tagLength a)
-
+noextract val finish: #a:alg -> acc a -> lbseq (tagLength a)
+ 
 // val hash2: #a:alg -> acc a -> b:bytes {length b % blockLength a = 0} -> acc a (decreases (length b))
 noextract let rec hash2 
   (#a:alg) 
@@ -114,6 +93,10 @@ noextract let rec hash2
   else
     let c,b = Seq.split b (blockLength a) in
     hash2 (compress v c) b
+
+
+let hash0 (#a:alg) (b:bseq {Seq.length b % blockLength a = 0}) = hash2 (acc0 #a) b
+
 
 (* PADDING AND LENGTH ENCODING *) 
 
@@ -137,14 +120,47 @@ val suffix: a:alg13 -> l:nat {l <= maxLength a} -> lbseq (suffixLength a l)
 
 let spec (a:alg13) (b:hashable a): lbseq (tagLength a) =
   let blocks = Seq.append b (suffix a (Seq.length b)) in
-  let acc = hash2 acc0 blocks in
+  let acc = hash0 blocks in
   let tag = finish acc in
   tag
 
+noextract 
+abstract 
+let hash (a:alg13) (b: hashable a): lbseq (tagLength a) = spec a b 
 
 (* ABSTRACT, EXTERNAL SPECIFICATION *) 
 
-(*abstract*) 
+/// 18-04-07 postponing verified integration with HACL* for now. We
+/// provide below a concise definition of the Merkle-Damgard
+/// construction. The plan is to integrate it with Benjamin's
+/// algorithmic specifications. At that point, we will probably hide
+/// the construction behind the provider interface (since we don't
+/// care about the construction when using or reasoning about them).
+
+// 18-04-07 
+(* 
+let lemma_blockLengths = 
+  assert_norm(
+    blockLength SHA256 == Spec.SHA2_256.size_block /\
+    blockLength SHA384 == Spec.SHA2_384.size_block /\
+    blockLength SHA512 == Spec.SHA2_512.size_block)
+
+noextract let lemma_tagLengths = 
+  assert_norm(
+    tagLength SHA256 == Spec.SHA2_256.size_hash /\
+    // truncated SHA512; note that `size_hash` is 64, not 48
+    tagLength SHA384 == Spec.SHA2_384.(size_word `op_Multiply` size_hash_final_w) /\
+    tagLength SHA512 == Spec.SHA2_512.size_hash)
+
+//#reset-options "--initial_ifuel 2 --initial_fuel 2 --z3rlimit 30"
+(* maximal input size, in bytes *)
+noextract let maxLength: alg -> nat = function
+  // 18-03-02 hacl-star uses a strict inequality; why?
+  | SHA256 -> Spec.SHA2_256.max_input_len_8 - 1 
+  | SHA384 -> Spec.SHA2_384.max_input_len_8 - 1 
+  | SHA512 -> Spec.SHA2_512.max_input_len_8 - 1
+  | _      -> pow2 61 (* conservative *)
+
 noextract 
 let hash (a:alg13) (b: hashable a): lbseq (tagLength a) = 
   match a with 
@@ -152,69 +168,48 @@ let hash (a:alg13) (b: hashable a): lbseq (tagLength a) =
   | SHA384 -> Spec.SHA2_384.hash b
   | SHA512 -> Spec.SHA2_512.hash b
 
-// TODO? I'd rather see Spec.Hash use the simpler style above than
-// write an inductive proof.
-
 val lemma_hash_spec: a:alg13 -> b: hashable a -> Lemma (hash a b = spec a b)
+*)
 
 
-(* ONE-SHOT IMPLEMENTATION; no need for an explicit bound since len <= 2^32 *)
+
+/// Next, we provide abstract interface to the stateful implementation, in 3 styles:
+///
+/// - a lower-level interface reflects the building blocks; they are
+///   used to build HMAC; they suffice to build the two other interfaces
+/// 
+/// - a simpler, one-shot interface for computing a hash
+/// 
+/// - a more flexible, incremental interface (WIP)
 
 type bptr = Buffer.buffer UInt8.t 
 let lbptr (l:nat)= b:bptr {Buffer.length b = l}
 let bptrlen (b:bptr) = len:UInt32.t {UInt32.v len = Buffer.length b}
 
-(* alternative seq, vec, ptr
-type uint8_s = Seq.seq UInt8.t
-type uint8_v = 
-type uint8_p = Buffer.buffer UInt8.t 
-*)
-
-val compute: 
-  a: alg13 -> 
-  len: UInt32.t -> 
-  input: lbptr (v len) -> 
-  output: lbptr (tagLength a){ Buffer.disjoint input output } -> Stack unit
-  (requires fun h0 -> 
-    Buffer.live h0 input /\ Buffer.live h0 output)
-  (ensures fun h0 () h1 -> 
-    Buffer.live h1 input /\ Buffer.live h1 output /\
-    Buffer.modifies_1 output h0 h1 /\
-    Buffer.as_seq h1 output = hash a (Buffer.as_seq h0 input))
-
-(* functional implementation wrapper *)
-
-// TODO missing BufferBytes here
-// val eval: a: alg13 -> b: Bytes.bytes -> Stack (Bytes.lbytes (tagLength a))
-//   (requires fun h -> True)
-//   (ensures fun h0 tag h1 -> Bytes.reveal tag = hash a (Bytes.reveal b) /\ h0 == h1)
-
-
-
-
-// TODO lowering the commented-out code in Hashing.fst 
-
-(* IMPLEMENTATION DETAILS supporting agile incremental hash, hmac, etc *)
+(* LOWER-LEVEL INTERFACE supporting agile incremental hash, hmac, etc *)
 
 // based on Crypto.HMAC, removing the agile_ prefixes
 
 (* convenient but a bit too concrete; the caller will allocate. See also the hack in Crypto.HMAC, and the need for disjointness. *)
 
+(* not any more: 
 // FIXME(adl): hash state allocation
 // The type of state a is a buffer of uint32 for SHA256
 // but a buffer of uint64 for SHA384 and SHA512
 // This is hard to do in KreMLin (see Crypto.Symmetric.PRF)
-// Instead we fake a u64[n] by allocation a u32[2*n]
+// For now, we fake a u64[n] by allocation a u32[2*n]
 // and rely on the implicit cast in C
+*)
+
 val state_size: alg13 -> UInt32.t 
 
 noextract 
 let state (a:alg13) =
   match a with
   | SHA256 -> b:Buffer.buffer UInt32.t {Buffer.length b = v (state_size SHA256)}
-  | SHA384 -> b:Buffer.buffer UInt64.t {Buffer.length b = v ( state_size SHA384)}
+  | SHA384 -> b:Buffer.buffer UInt64.t {Buffer.length b = v (state_size SHA384)}
   | SHA512 -> b:Buffer.buffer UInt64.t {Buffer.length b = v (state_size SHA512)}
-val as_acc: #a:alg13 -> h:FStar.HyperStack.mem -> state a -> acc a 
+val as_acc: #a:alg13 -> h:FStar.HyperStack.mem -> state a -> acc a
 
 val init:
   a:alg13 -> 
@@ -223,7 +218,7 @@ val init:
   (ensures fun h0 () h1 -> 
     Buffer.live #(if a = SHA256 then UInt32.t else UInt64.t) h1 st /\
     Buffer.modifies_1 #(if a = SHA256 then UInt32.t else UInt64.t) st h0 h1  /\ 
-    as_acc h1 st = acc0)
+    as_acc h1 st == acc0 #a)
 
 val update:
   a:alg13 -> 
@@ -237,7 +232,36 @@ val update:
     Buffer.live #(if a = SHA256 then UInt32.t else UInt64.t) h1 st /\ 
     Buffer.live h1 block /\
     Buffer.modifies_1 #(if a = SHA256 then UInt32.t else UInt64.t) st h0 h1 /\ 
-    as_acc h1 st = compress (as_acc h0 st) (Buffer.as_seq h0 block))
+    as_acc h1 st == compress (as_acc h0 st) (Buffer.as_seq h0 block))
+
+
+let rec lemma_hash2 
+  (#a: alg) 
+  (a0: acc a)
+  (b0 b1: (b:bseq{ Seq.length b % blockLength a = 0})): 
+  Tot 
+    (_:unit{hash2 a0 (Seq.append b0 b1) == hash2 (hash2 a0 b0) b1})
+    (decreases (Seq.length b0)) 
+=
+  if Seq.length b0 = 0 then (
+    Seq.lemma_empty b0;
+    Seq.append_empty_l b1 )
+  else (
+    let c,b0' = Seq.split b0 (blockLength a) in
+    let c',b' = Seq.split (Seq.append b0 b1) (blockLength a) in
+    Seq.append_assoc c b0' b1;
+    //Seq.lemma_split b0 (blockLength a);
+    //Seq.lemma_eq_intro (Seq.append b0 b1) (Seq.append c' b');
+    Seq.lemma_eq_intro c c';
+    Seq.lemma_eq_intro b' (Seq.append b0' b1);
+    lemma_hash2 (hash2 a0 c) b0' b1)
+
+let lemma_compress 
+  (#a: alg) 
+  (a0: acc a)
+  (c: lbseq (blockLength a)): 
+  Lemma (compress a0 c == hash2 a0 c) = ()
+
 
 // 18-03-03 update_multi is a parametric loop best left to the
 // caller---unless we expect it to be further optimized.
@@ -255,7 +279,7 @@ val update_multi:
     Buffer.live #(if a = SHA256 then UInt32.t else UInt64.t) h1 st /\ 
     Buffer.live h1 blocks /\
     Buffer.modifies_1 #(if a = SHA256 then UInt32.t else UInt64.t) st h0 h1 /\ 
-    as_acc h1 st = hash2 (as_acc h0 st) (Buffer.as_seq h0 blocks))
+    as_acc h1 st == hash2 (as_acc h0 st) (Buffer.as_seq h0 blocks))
 
 // 18-03-05 note the *new length-passsing convention*
 // 18-03-03 it would be simpler to let the caller keep track of lengths!
@@ -264,20 +288,25 @@ val update_last:
   a:alg13 -> 
   st:state a -> 
   last: bptr {Buffer.length last <= blockLength a /\ Buffer.disjoint #(if a = SHA256 then UInt32.t else UInt64.t) st last} -> 
-  total_len: UInt32.t {Buffer.length last = v total_len % blockLength a} ->
+  total_len: UInt32.t {
+    let l = v total_len in 
+    l <= maxLength a /\ 
+    Buffer.length last = l % blockLength a } ->
   Stack unit 
   (requires fun h0 -> 
     Buffer.live #(if a = SHA256 then UInt32.t else UInt64.t) h0 st /\ Buffer.live h0 last)
   (ensures fun h0 () h1 -> 
     Buffer.live #(if a = SHA256 then UInt32.t else UInt64.t) h1 st /\ Buffer.live h1 last /\
     Buffer.modifies_1 #(if a = SHA256 then UInt32.t else UInt64.t) st h0 h1 /\ 
-    ( let l1 = v total_len % blockLength a in
-      let l0 = v total_len - l1 in 
-      forall (prior: lbseq l0). 
-      ( as_acc h0 st = hash2 acc0 prior ==>
-        finish (as_acc h1 st) = spec a (Seq.append prior (Buffer.as_seq h0 last)) )))
+    as_acc h1 st == hash2 (as_acc h0 st) (Seq.append (Buffer.as_seq h0 last) (suffix a (v total_len))))
+      
+// forall (prior: lbseq l0).{:pattern (as_acc h0 st == hash2 (acc0 #a) prior)} 
+// ( as_acc h0 st == hash2 acc0 prior ==>
+// finish #a (as_acc h1 st) == spec a (Seq.append prior (Buffer.as_seq h0 last)) ))))
 
-// for HSL we'll need a variant that copies, finalizes, and extracts.
+// for HandshakeLog we will need a variant that copies the state,
+// finalizes, and extracts to compute successive hashes of the
+// transcript.
 
 // 18-03-03 can't also be named finished
 val extract: 
@@ -291,6 +320,33 @@ val extract:
     Buffer.live #(if a = SHA256 then UInt32.t else UInt64.t) h1 st /\ Buffer.live h1 output /\
     Buffer.modifies_1 output h0 h1 /\ 
     Buffer.as_seq h1 output = finish (as_acc h0 st))
+
+
+
+(* ONE-SHOT IMPLEMENTATION; implementatable from the lower-level
+interface above. No need for an explicit bound since len <= 2^32 *)
+
+(* alternative seq, vec, ptr
+type uint8_s = Seq.seq UInt8.t
+type uint8_v = 
+type uint8_p = Buffer.buffer UInt8.t 
+*)
+
+val compute: 
+  a: alg13 -> 
+  len: UInt32.t -> 
+  input: lbptr (v len) -> 
+  output: lbptr (tagLength a){ Buffer.disjoint input output } -> Stack unit
+  (requires fun h0 -> 
+    Buffer.live h0 input /\ Buffer.live h0 output)
+  (ensures fun h0 () h1 -> 
+    Buffer.live h1 input /\ Buffer.live h1 output /\
+    Buffer.modifies_1 output h0 h1 /\
+    v len <= maxLength a /\ (* required for subtyping the RHS below *)
+    Buffer.as_seq h1 output = hash a (Buffer.as_seq h0 input))
+
+
+(* TODO a third, incremental-hash implementation. *)
 
 /// INCREMENTAL HASHING (working notes)
 /// The state includes
@@ -318,3 +374,17 @@ val extract:
 /// of the stack before finishing.
 ///
 /// Can we get the compression function and the loop coded in VALE?
+
+
+
+/// We finally provide high-level-bytes implementation wrappers.
+/// (currently used for idealization in secure_api and TLS
+/// 
+(* functional implementation wrapper *)
+
+// TODO missing BufferBytes here
+// val eval: a: alg13 -> b: Bytes.bytes -> Stack (Bytes.lbytes (tagLength a))
+//   (requires fun h -> True)
+//   (ensures fun h0 tag h1 -> Bytes.reveal tag = hash a (Bytes.reveal b) /\ h0 == h1)
+
+
